Proof that the representaiton of integers for arithmetic is injective.

Coq/Simplicity/Arith.v
@@ -1,15 +1,68 @@
 Require Import Simplicity.Ty.
 Require Import Simplicity.Alg.
 Require Import Simplicity.Bit.
+Require Import ZArith.
 
+Local Set Keyed Unification.
 Local Open Scope ty_scope.
 Local Open Scope term_scope.
+Local Open Scope core_alg_scope.
 
 Fixpoint Word (n : nat) :=
 match n with
 | 0 => Bit
 | S n => let rec := Word n in Prod rec rec
 end.
+
+Module ToZ.
+
+Module Class.
+Record class T := Class { toZ : T -> Z; bitSize : nat }.
+End Class.
+Structure type := Pack { obj : Ty; class_of : Class.class obj }.
+
+Module Ops.
+Definition toZ {T : type} : obj T -> Z :=
+ let '(Pack _ (Class.Class _ f _)) := T in f.
+Definition bitSize (T : type) : nat :=
+ let '(Pack _ (Class.Class _ _ n)) := T in n.
+Coercion obj : type >-> Ty.
+Coercion class_of : type >-> Class.class.
+End Ops.
+
+End ToZ.
+Import ToZ.Ops.
+
+Definition BitToZ_Class := ToZ.Class.Class (Word 0) (fun bit => match bit with | inl _ => 0%Z | inr _ => 1%Z end) 1.
+Canonical Structure BitToZ : ToZ.type := Eval compute in ToZ.Pack Bit BitToZ_Class.
+
+Definition PairToZ_Class {a b : Ty} (a_class : ToZ.Class.class a) (b_class : ToZ.Class.class b) :
+  ToZ.Class.class (a * b) :=
+ToZ.Class.Class (a * b) (fun p =>
+  let (a, b) := p in
+  ToZ.Class.toZ _ a_class a * (two_power_nat (ToZ.Class.bitSize _ b_class)) + ToZ.Class.toZ _ b_class b)%Z
+  (ToZ.Class.bitSize _ a_class + ToZ.Class.bitSize _ b_class).
+Canonical Structure PairToZ (a b : ToZ.type) : ToZ.type := ToZ.Pack (a * b) (PairToZ_Class a b).
+
+Fixpoint WordToZ_Class {n : nat} : ToZ.Class.class (Word n) :=
+match n with
+| 0 => BitToZ_Class
+| (S m) => PairToZ_Class WordToZ_Class WordToZ_Class
+end.
+Canonical Structure WordToZ (n : nat) : ToZ.type := ToZ.Pack (Word n) WordToZ_Class.
+
+Lemma toZ_Pair {A B : ToZ.type} (a : A) (b : B) :
+  @toZ (PairToZ A B) (a, b) = (toZ a * two_power_nat (bitSize B) + toZ b)%Z.
+Proof.
+destruct A; destruct B; reflexivity.
+Qed.
+
+Lemma bitSize_Pair (A B : ToZ.type) :
+  bitSize (PairToZ A B) = (bitSize A + bitSize B)%nat.
+Proof.
+destruct A; destruct B; reflexivity.
+Qed.
+
 
 Section Definitions.
 
@@ -84,6 +137,127 @@ match n with
 end.
 
 End Definitions.
+
+Lemma fullAdder_correct n : forall (a b : Word n) (c : Bit),
+  (toZ (|[fullAdder]| ((a, b), c)) = toZ a + toZ b  + toZ c)%Z.
+Proof.
+induction n.
+ intros [[] | []] [[] | []] [[] | []]; reflexivity.
+intros [ahi alo] [bhi blo] c.
+cbn -[toZ]; fold tySem; fold (tySem Bit).
+rewrite (toZ_Pair ahi alo), (toZ_Pair bhi blo).
+set (C := two_power_nat _).
+transitivity ((toZ ahi + toZ bhi) * C + (toZ alo + toZ blo + toZ c))%Z;[|ring].
+rewrite <- IHn.
+destruct (|[fullAdder]| (alo, blo, c)) as [c0 rlo]; clear alo blo c.
+cbn [fst snd].
+rewrite (toZ_Pair c0 rlo).
+fold C.
+transitivity ((toZ ahi + toZ bhi + toZ c0) * C + toZ rlo)%Z;[|ring].
+rewrite <- IHn.
+destruct (|[fullAdder]| (ahi, bhi, c0)) as [c1 rhi]; clear ahi bhi c0.
+cbn [fst snd].
+rewrite (toZ_Pair c1 rhi); fold C.
+rewrite (toZ_Pair c1 _).
+rewrite (bitSize_Pair (WordToZ n) (WordToZ n)).
+rewrite two_power_nat_correct, Zpower_nat_is_exp, <- two_power_nat_correct; fold C.
+rewrite (toZ_Pair rhi rlo); fold C.
+ring.
+Qed.
+
+Lemma adder_correct n : forall (a b : Word n),
+  (toZ (|[adder]| (a, b)) = toZ a + toZ b)%Z.
+induction n.
+ intros [[] | []] [[] | []]; reflexivity.
+intros [ahi alo] [bhi blo].
+cbn -[toZ]; fold tySem; fold (tySem Bit).
+rewrite (toZ_Pair ahi alo), (toZ_Pair bhi blo).
+set (C := two_power_nat _).
+transitivity ((toZ ahi + toZ bhi) * C + (toZ alo + toZ blo))%Z;[|ring].
+rewrite <- (IHn alo).
+destruct (|[adder]| (alo, blo)) as [c0 rlo]; clear alo blo.
+cbn [fst snd].
+rewrite (toZ_Pair c0 rlo).
+fold C.
+transitivity ((toZ ahi + toZ bhi + toZ c0) * C + toZ rlo)%Z;[|ring].
+rewrite <- fullAdder_correct.
+destruct (|[fullAdder]| (ahi, bhi, c0)) as [c1 rhi]; clear ahi bhi c0.
+cbn [fst snd].
+rewrite (toZ_Pair c1 rhi); fold C.
+rewrite (toZ_Pair c1 _).
+rewrite (bitSize_Pair (WordToZ n) (WordToZ n)).
+rewrite two_power_nat_correct, Zpower_nat_is_exp, <- two_power_nat_correct; fold C.
+rewrite (toZ_Pair rhi rlo); fold C.
+ring.
+Qed.
+
+Lemma fullMultiplier_correct n : forall (a b c d : Word n),
+  (toZ (|[fullMultiplier]| ((a, b), (c, d))) = toZ a * toZ b + toZ c + toZ d)%Z.
+Proof.
+induction n.
+ intros [[] | []] [[] | []] [[] | []] [[] | []]; reflexivity.
+intros [ahi alo] [bhi blo] [chi clo] [dhi dlo].
+cbn -[toZ]; fold tySem; fold (tySem Bit).
+rewrite (toZ_Pair ahi alo), (toZ_Pair bhi blo), (toZ_Pair chi clo), (toZ_Pair dhi dlo).
+set (C := two_power_nat _).
+transitivity ((toZ ahi * C + toZ alo) * toZ bhi * C +
+ ((toZ ahi * toZ blo + toZ chi + toZ dhi) * C) + (toZ alo * toZ blo + toZ clo + toZ dlo))%Z;
+ [|ring].
+rewrite <- 2!IHn.
+destruct (|[fullMultiplier]| ((alo, blo), (clo, dlo))) as [c0 rOO]; clear clo dlo.
+destruct (|[fullMultiplier]| ((ahi, blo), (chi, dhi))) as [c1 c2]; clear chi dhi blo.
+cbn [fst snd].
+rewrite (toZ_Pair c1 c2), (toZ_Pair c0 rOO); fold C.
+transitivity ((toZ ahi * toZ bhi + toZ c1) * C * C +
+ (toZ bhi * toZ alo + toZ c2 + toZ c0) * C + toZ rOO)%Z;
+ [|ring].
+rewrite <- IHn.
+destruct (|[fullMultiplier]| ((bhi, alo), (c2, c0))) as [c3 rOI]; clear c2 c0 alo.
+cbn [fst snd].
+rewrite (toZ_Pair c3 rOI); fold C.
+transitivity ((toZ ahi * toZ bhi + toZ c3 + toZ c1) * C * C + toZ rOI * C + toZ rOO)%Z;
+ [|ring].
+rewrite <- IHn.
+destruct (|[fullMultiplier]| ((ahi, bhi), (c3, c1))) as [rII rIO]; clear c3 c1 ahi bhi.
+rewrite toZ_Pair, (toZ_Pair rOI rOO); fold C.
+rewrite (bitSize_Pair (WordToZ n) (WordToZ n)).
+rewrite two_power_nat_correct, Zpower_nat_is_exp, <- two_power_nat_correct; fold C.
+set (X := toZ _); ring.
+Qed.
+
+Lemma multiplier_correct n : forall (a b : Word n),
+  (toZ (|[multiplier]| (a, b)) = toZ a * toZ b)%Z.
+Proof.
+induction n.
+ intros [[] | []] [[] | []]; reflexivity.
+intros [ahi alo] [bhi blo].
+cbn -[toZ]; fold tySem; fold (tySem Bit).
+rewrite (toZ_Pair ahi alo), (toZ_Pair bhi blo).
+set (C := two_power_nat _).
+transitivity ((toZ ahi * C + toZ alo) * toZ bhi * C +
+ ((toZ ahi * toZ blo) * C) + (toZ alo * toZ blo))%Z;
+ [|ring].
+rewrite <- 2!IHn.
+destruct (|[multiplier]| (alo, blo)) as [c0 rOO].
+destruct (|[multiplier]| (ahi, blo)) as [c1 c2]; clear blo.
+cbn [fst snd].
+rewrite (toZ_Pair c1 c2), (toZ_Pair c0 rOO); fold C.
+transitivity ((toZ ahi * toZ bhi + toZ c1) * C * C +
+ (toZ bhi * toZ alo + toZ c2 + toZ c0) * C + toZ rOO)%Z;
+ [|ring].
+rewrite <- fullMultiplier_correct.
+destruct (|[fullMultiplier]| ((bhi, alo), (c2, c0))) as [c3 rOI]; clear c2 c0 alo.
+cbn [fst snd].
+rewrite (toZ_Pair c3 rOI); fold C.
+transitivity ((toZ ahi * toZ bhi + toZ c3 + toZ c1) * C * C + toZ rOI * C + toZ rOO)%Z;
+ [|ring].
+rewrite <- fullMultiplier_correct.
+destruct (|[fullMultiplier]| ((ahi, bhi), (c3, c1))) as [rII rIO]; clear c3 c1 ahi bhi.
+rewrite toZ_Pair, (toZ_Pair rOI rOO); fold C.
+rewrite (bitSize_Pair (WordToZ n) (WordToZ n)).
+rewrite two_power_nat_correct, Zpower_nat_is_exp, <- two_power_nat_correct; fold C.
+set (X := toZ _); ring.
+Qed.
 
 Lemma adderBit_Parametric {term1 term2 : Core.type} (R : Core.ReynoldsRel term1 term2) : R _ _ adderBit adderBit.
 Proof.
